alloc () almost done in Steel.HigherArray
some weird bug

src/Steel.Array.fsti
@@ -1,8 +1,8 @@
 module Steel.Array
 
-//open FStar.Ghost
-//open Steel.Effect.Atomic
-//open Steel.Effect
+open FStar.Ghost
+open Steel.Effect.Atomic
+open Steel.Effect
 //open FStar.Real
 //open FStar.PCM
 open Steel.FractionalPermission
@@ -28,7 +28,7 @@ let is_null (#a: Type0) (#n: nat)
   = H.is_null #(U.raise_t a) #n
 
 let pts_to_sl (#a: Type0)
-  (n: nat)
+  (#n: nat)
   (r: array_ref a #n)
   (i1: nat)
   (i2: nat{i1 < i2 /\ i2 <= n})
@@ -86,8 +86,8 @@ let pts_to_ref_injective (#a: Type0) (#n: nat)
   (m:Mem.mem)
   : Lemma
     (requires Mem.interp (
-      pts_to_sl n r i1 i2 p1 subv1 `Mem.star`
-      pts_to_sl n r i1 i2 p2 subv2) m)
+      pts_to_sl r i1 i2 p1 subv1 `Mem.star`
+      pts_to_sl r i1 i2 p2 subv2) m)
     (ensures subv1 == subv2)
   =
   map_seq_len U.raise_val subv1;
@@ -104,7 +104,7 @@ let pts_to_not_null (#a:Type0) (#n: nat)
   (p: lseq perm n)
   (subv: lseq a (i2 - i1 + 1))
   (m:Mem.mem)
-  : Lemma (requires Mem.interp (pts_to_sl n r i1 i2 p subv) m)
+  : Lemma (requires Mem.interp (pts_to_sl r i1 i2 p subv) m)
           (ensures r =!= null)
   =
   map_seq_len U.raise_val subv;
@@ -120,8 +120,8 @@ let aux_sl (#a: Type0) (#n: nat)
   (m:Mem.mem)
   : Lemma
   (requires
-    Mem.interp (pts_to_sl n r i1 i2 p subv1) m /\
-    Mem.interp (pts_to_sl n r i1 i2 p subv2) m
+    Mem.interp (pts_to_sl r i1 i2 p subv1) m /\
+    Mem.interp (pts_to_sl r i1 i2 p subv2) m
   )
   (ensures subv1 == subv2)
   =
@@ -147,7 +147,7 @@ let pts_to_witinv (#a:Type) (#n: nat)
   (i2: nat{i1 < i2 /\ i2 < n})
   (p: lseq perm n)
   : Lemma (Mem.is_witness_invariant (
-      pts_to_sl n r i1 i2 p
+      pts_to_sl r i1 i2 p
     ))
   =
   Classical.forall_intro_3 (
@@ -155,3 +155,53 @@ let pts_to_witinv (#a:Type) (#n: nat)
       aux_sl r i1 i2 p
     )
   )
+
+let pts_to (#a: Type) (#n: nat)
+  (r: array_ref a #n)
+  (i1: nat)
+  (i2: nat{i1 < i2 /\ i2 <= n})
+  ([@@@smt_fallback] p: lseq perm n)
+  ([@@@smt_fallback] subv: lseq a (i2 - i1 + 1))
+  : vprop
+  = to_vprop (pts_to_sl r i1 i2 p subv)
+
+let pts_to_injectiv_eq (#a: Type)
+  (#n: nat)
+  (#opened:Mem.inames)
+  (r: array_ref a #n)
+  (i1: nat)
+  (i2: nat{i1 < i2 /\ i2 < n})
+  (p1 p2: lseq perm n)
+  (subv1 subv2: lseq a (i2 - i1 + 1))
+  : SteelGhost unit opened
+  (pts_to r i1 i2 p1 subv1 `star`
+   pts_to r i1 i2 p2 subv2)
+  (fun _ -> pts_to r i1 i2 p1 subv1 `star`
+   pts_to r i1 i2 p2 subv1)
+  (requires fun _ -> True)
+  (ensures fun _ _ _ -> subv1 == subv2)
+  =
+  extract_info_raw
+    (pts_to r i1 i2 p1 subv1 `star`
+     pts_to r i1 i2 p2 subv2)
+    (subv1 == subv2)
+    (fun m -> pts_to_ref_injective r i1 i2 p1 p2 subv1 subv2 m);
+  rewrite_slprop
+    (pts_to r i1 i2 p2 subv2)
+    (pts_to r i1 i2 p2 subv1)
+    (fun _ -> ())
+
+let mk_perm (n: nat) (p: perm)
+  = Seq.create n p
+
+let alloc_pt (#a: Type)
+  (n: nat)
+  (v: lseq a n)
+  : Steel
+  (array_ref a #n)
+  emp
+  (fun r -> pts_to r 0 (n-1) (mk_perm n (Some full_perm)) v)
+  (requires fun _ -> True)
+  (ensures fun _ r _ -> not (is_null r))
+  =
+  admit ()
